Phi_System/IDE_CP_Reasoning1.thy
@@ -55,24 +55,6 @@ text \<open>Annotate a rule generated during the programming, to differentiate f
   contextual facts. The normal facts are stored in \<open>\<phi>lemmata\<close> while the generated rules
   are in \<open>\<phi>generated\<close> (or maybe a better name like \<phi>generated_rules?)\<close>
 
-(*TODO: explain*)
-(*TODO: polish*)
-
-(*definition SMorphism :: \<open>'a \<Rightarrow> 'a\<close> ("SMORPH _" [17] 16) (*TODO: rename it, maybe like SP standing for 
-                                                          Structural Preserving*)
-  where [iff]: \<open>SMorphism X = X\<close>
-*)
-definition Generated_Rule :: \<open>mode \<Rightarrow> bool \<Rightarrow> bool \<Rightarrow> bool\<close>
-  where \<open>Generated_Rule _ embedded_prems stuff = (embedded_prems \<longrightarrow> stuff)\<close>
-
-(*consts morphism_mode :: mode (*TODO: depreciate*)*)
-
-(*abbreviation Automatic_Rule :: \<open>bool \<Rightarrow> bool \<Rightarrow> bool\<close> where \<open>Automatic_Rule \<equiv> Generated_Rule (MODE_AUTO default)\<close>*)
-
-(*consts REVERSE_TRANSFORMATION :: mode
-abbreviation Reverse_Transformation :: \<open>bool \<Rightarrow> bool \<Rightarrow> bool\<close>
-  where \<open>Reverse_Transformation \<equiv> Generated_Rule (MODE_AUTO REVERSE_TRANSFORMATION)\<close>
-*)
 
 text \<open>TODO: update this
 
